\title{Proof Checker Notes}
\author{Yu-Yang Lin}
\date{\today}

\documentclass[twoside,a4paper]{article}

\usepackage{natbib}
\usepackage{mathtools}
\usepackage{syntax}
\usepackage{bussproofs}
\usepackage{boxproof}
\usepackage[margin=2cm]{geometry}
\usepackage{changepage}

\usepackage[utf8]{inputenc}
\usepackage[english]{babel}
\setlength{\parskip}{1em}
\setlength\parindent{0pt}

% Palatino for rm and math | Helvetica for ss | Courier for tt
\usepackage{mathpazo} % math & rm
\linespread{1.05} % Palatino needs more leading (space between lines)
\usepackage[scaled]{helvet} %
\usepackage{courier} % tt
\normalfont
\usepackage[T1]{fontenc}

\usepackage{amsthm}
\usepackage{amssymb}
\theoremstyle{definition}
\newtheorem{definition}{Definition}

%NEW quantifier (fresh)
\usepackage{graphics} %needed for the NEW quantifier
\newcommand\new[0]{\reflectbox{\ensuremath{\mathsf{N}}}}
%The quantifier itself, a reversed sans-serif N
%(by analogy with the reversed E of `exists'
%and the reversed A of `forall')
\newcommand\New[1]{\new #1.}
%A macro, as in \New{a}\phi

\begin{document}
\maketitle

\section{Syntax Grammar}
\begin{center}
\begin{tabular}{rll}
(types)& $\tau$ ::= bool
| $\tau$ $\rightarrow$ $\tau $ | nat | list $\tau$
\\
(hypotheses)& A , B ::= $\top$ | $\bot$
| A $\wedge$ B | A $\vee$ B | A $\supset$ B
| $\forall$ $x$ : $\tau$ . A | $\exists$ $x$ : $\tau$ . A
| t = t : $\tau$
\\
(terms)& e , t ::= $x$ | t t | true | false
| [ ] | t :: t  %lists
| zero | suc( t ) %natural numbers
\\
(term context)& $\psi$ ::= . | $\psi$, $x$ : $\tau$
\end{tabular}

\begin{tabular}{rll}
$\psi$ &$\vdash$ & t : $\tau$\\
$\psi$ &$\vdash$ & A prop
\end{tabular}
\end{center}

\section{Specification rules for terms and propositional hypotheses}

Note: functions are included as term types, but not directly as term constructors. Instead, function terms are added into the term context ($\psi$) manually. This simplifies the checker since function type inference is not required.

\subsection{Terms}
Natural Numbers:
\[
\AxiomC{}
\RightLabel{\quad (nat-zero)}
\UnaryInfC{$\psi \vdash$ zero : nat}
\DisplayProof
\qquad
\qquad
\AxiomC{$\psi \vdash$ t : nat}
\RightLabel{\quad (nat-suc-n)}
\UnaryInfC{$\psi \vdash$ suc( t ) : nat}
\DisplayProof
\]

Booleans:
\[
\AxiomC{}
\RightLabel{\quad (bool-true)}
\UnaryInfC{$\psi \vdash$ true : bool}
\DisplayProof
\qquad
\qquad
\AxiomC{}
\RightLabel{\quad (bool-false)}
\UnaryInfC{$\psi \vdash$ false : bool}
\DisplayProof
\]

Lists:
\[
\AxiomC{}
\RightLabel{\quad (list-nil)}
\UnaryInfC{$\psi \vdash$ [ ] : list t}
\DisplayProof
\qquad
\qquad
\AxiomC{$\psi \vdash$ t' : t}
\AxiomC{$\psi \vdash$ t'' : list t}
\RightLabel{\quad (list-cons)}
\BinaryInfC{$\psi \vdash$ t' :: t'' : list t}
\DisplayProof
\]

Variables:
\[
\AxiomC{$x : \tau \in \psi$}
\RightLabel{\quad (var)}
\UnaryInfC{$\psi \vdash x : \tau$}
\DisplayProof
\]

Application:
\[
\AxiomC{$\psi \vdash$ t : $\tau \rightarrow \tau$'}
\AxiomC{$\psi \vdash$ t' : $\tau$}
\RightLabel{\quad (app)}
\BinaryInfC{$\psi \vdash$ t t' : $\tau$'}
\DisplayProof
\]

\subsection{Propositions}
Truth and Falsity Propositions:
\[
\AxiomC{}
\RightLabel{\quad ($\top$-prop)}
\UnaryInfC{$\psi \vdash$ $\top$  prop}
\DisplayProof
\qquad
\qquad
\AxiomC{}
\RightLabel{\quad ($\bot$-prop)}
\UnaryInfC{$\psi \vdash$ $\bot$  prop}
\DisplayProof
\]

Binary Relation Propositions:
\[
\AxiomC{$\psi \vdash$ A prop}
\AxiomC{$\psi \vdash$ B prop}
\RightLabel{\quad ($\wedge$-prop)}
\BinaryInfC{$\psi \vdash$ A $\wedge$ B prop}
\DisplayProof
\]

\[
\AxiomC{$\psi \vdash$ A prop}
\AxiomC{$\psi \vdash$ B prop}
\RightLabel{\quad ($\vee$-prop)}
\BinaryInfC{$\psi \vdash$ A $\vee$ B prop}
\DisplayProof
\]

\[
\AxiomC{$\psi \vdash$ A prop}
\AxiomC{$\psi \vdash$ B prop}
\RightLabel{\quad ($\supset$-prop)}
\BinaryInfC{$\psi \vdash$ A $\supset$ B prop}
\DisplayProof
\]

\[
\AxiomC{$\psi \vdash $t$ : \tau$}
\AxiomC{$\psi \vdash $t'$ : \tau$}
\RightLabel{\quad (eq-prop)}
\BinaryInfC{$\psi \vdash$ (t = t' : $\tau$) prop}
\DisplayProof
\]

Quantifier Propositions:
\[
\AxiomC{$\psi , x : \tau \vdash$ A prop}
\RightLabel{\quad ($\forall$-prop)}
\UnaryInfC{$\psi \vdash \forall x : \tau .$ A prop}
\DisplayProof
\]

\[
\AxiomC{$\psi , x : \tau \vdash$ A prop}
\RightLabel{\quad ($\exists$-prop)}
\UnaryInfC{$\psi \vdash \exists x : \tau .$ A prop}
\DisplayProof
\]

\section{Implementation rules for type inference and checking}

\subsection{Syntax grammar}
\begin{center}
\begin{tabular}{rll}
(infer)& e ::= x
| e v | true | false | zero | suc( e )
\\
(check)& v ::= v :: v  | nil | e
\end{tabular}
\end{center}

Type Inferece Rule:
\[\overset{-}\psi \vdash \overset{-}{t} \Rightarrow \overset{+}\tau\]

Type Checking Rule:
\[\overset{-}\psi \vdash \overset{-}{t} \Leftarrow \overset{-}\tau\]

\subsection{Term type inference}
Variables:
\[
\AxiomC{$x : \tau \in \psi$}
\RightLabel{\quad (var)}
\UnaryInfC{$\psi \vdash x \Rightarrow \tau$}
\DisplayProof
\]

Application:
\[
\AxiomC{$\psi \vdash$ t $\Rightarrow$ $\tau \rightarrow \tau$'}
\AxiomC{$\psi \vdash$ t' $\Leftarrow$ $\tau$}
\RightLabel{\quad (app)}
\BinaryInfC{$\psi \vdash$ t t' $\Rightarrow$ $\tau$'}
\DisplayProof
\]

Natural Numbers:
\[
\AxiomC{}
\RightLabel{\quad (nat-zero)}
\UnaryInfC{$\psi \vdash$ zero $\Rightarrow$ nat}
\DisplayProof
\qquad
\qquad
\AxiomC{$\psi \vdash$ t $\Leftarrow$ nat}
\RightLabel{\quad (nat-suc-n)}
\UnaryInfC{$\psi \vdash$ suc( t ) $\Rightarrow$ nat}
\DisplayProof
\]

Booleans:
\[
\AxiomC{}
\RightLabel{\quad (bool-true)}
\UnaryInfC{$\psi \vdash$ true $\Rightarrow$ bool}
\DisplayProof
\qquad
\qquad
\AxiomC{}
\RightLabel{\quad (bool-false)}
\UnaryInfC{$\psi \vdash$ false $\Rightarrow$ bool}
\DisplayProof
\]

\subsection{Term type checking}
Lists:
\[
\AxiomC{}
\RightLabel{\quad (list-nil)}
\UnaryInfC{$\psi \vdash$ [ ] $\Leftarrow$ list t}
\DisplayProof
\qquad
\qquad
\AxiomC{$\psi \vdash$ t' $\Leftarrow$ t}
\AxiomC{$\psi \vdash$ t'' $\Leftarrow$ list t}
\RightLabel{\quad (list-cons)}
\BinaryInfC{$\psi \vdash$ t' :: t'' $\Leftarrow$ list t}
\DisplayProof
\]

Inference Case:
\[
\AxiomC{$\psi \vdash$ t $\Rightarrow \tau$'}
\AxiomC{$\tau = \tau'$}
\RightLabel{\quad (app)}
\BinaryInfC{$\psi \vdash$ t $\Leftarrow$ $\tau$}
\DisplayProof
\]

\subsection{Propositions type checking}
Truth and Falsity Propositions:
\[
\AxiomC{}
\RightLabel{\quad ($\top$-prop)}
\UnaryInfC{$\psi \vdash$ $\top$ prop}
\DisplayProof
\qquad
\qquad
\AxiomC{}
\RightLabel{\quad ($\bot$-prop)}
\UnaryInfC{$\psi \vdash$ $\bot$ prop}
\DisplayProof
\]

Binary Relation Propositions:
\[
\AxiomC{$\psi \vdash$ A prop}
\AxiomC{$\psi \vdash$ B prop}
\RightLabel{\quad ($\wedge$-prop)}
\BinaryInfC{$\psi \vdash$ A $\wedge$ B prop}
\DisplayProof
\]

\[
\AxiomC{$\psi \vdash$ A prop}
\AxiomC{$\psi \vdash$ B prop}
\RightLabel{\quad ($\vee$-prop)}
\BinaryInfC{$\psi \vdash$ A $\vee$ B prop}
\DisplayProof
\]

\[
\AxiomC{$\psi \vdash$ A prop}
\AxiomC{$\psi \vdash$ B prop}
\RightLabel{\quad ($\supset$-prop)}
\BinaryInfC{$\psi \vdash$ A $\supset$ B prop}
\DisplayProof
\]

\[
\AxiomC{$\psi \vdash $t$ \Leftarrow \tau$}
\AxiomC{$\psi \vdash $t'$ \Leftarrow \tau$}
\RightLabel{\quad (eq-prop)}
\BinaryInfC{$\psi \vdash$ (t = t' $\Leftarrow$ $\tau$) prop}
\DisplayProof
\]

Quantifier Propositions:
\[
\AxiomC{$\psi , x \Leftarrow \tau \vdash$ A prop}
\RightLabel{\quad ($\forall$-prop)}
\UnaryInfC{$\psi \vdash \forall x \Leftarrow \tau .$ A prop}
\DisplayProof
\]

\[
\AxiomC{$\psi , x \Leftarrow \tau \vdash$ A prop}
\RightLabel{\quad ($\exists$-prop)}
\UnaryInfC{$\psi \vdash \exists x \Leftarrow \tau .$ A prop}
\DisplayProof
\]

\subsection{Function signatures}
\begin{center}
\tt
\begin{tabular} {rl}
infer_term &: $\psi$ $\rightarrow$ t $\rightarrow$ $\tau$ option
\\
check_term &: $\psi$ $\rightarrow$ t $\rightarrow$ $\tau$ $\rightarrow$ unit option
\\
check_prop &: $\psi$ $\rightarrow$ A $\rightarrow$ unit option
\end{tabular}

\begin{tabular} {rll}

&val infer_term &: ctx -> term -> tp option
\\
&val check_term &: ctx -> term -> tp -> unit option
\\
&val check_prop &: ctx -> prop -> unit option

\end{tabular}
\end{center}


\section{Well-formedness of proofs}
\subsection{Syntax grammar}
\begin{center}
\begin{tabular}{rrrl}
(proofs)& p , q &::=& by H
\\ &&|& (p , q)
\\ &&|& let (H',H'') = H in p
\\ &&|& (p , q ) either
\\ &&|& match [H] : (A $\vee$ B) with (
\\ &&&\qquad \qquad | A [H']: p -> C
\\ &&&\qquad \qquad | B [H'']: q -> C )
\\
(hypotheses context)& $\Gamma$ &::=& \quad $\cdot$ \quad
\\ &&| & $\Gamma$ , H : A
\\ &&| & Assume A [ H ] , p
\end{tabular}

\begin{tabular} {rl}
$\psi ; \Gamma$ &$\vdash$ p : A
\\
$\psi $ & $\vdash \Gamma$
\end{tabular}
\end{center}

\subsection{Rules}
Truth and Falsity:
\[
\AxiomC{}
\RightLabel{\quad ($\top$R)}
\UnaryInfC{$\psi ; \Gamma \vdash$ tt : $\top$}
\DisplayProof
\qquad
\qquad
\AxiomC{}
\RightLabel{\quad ($\bot$L)}
\UnaryInfC{$\psi ; \Gamma ,$  [H] : $\bot$
$\vdash $
Absurd H : C
}
\DisplayProof
\]

Conjunction:
\[
\AxiomC{$\psi ; \Gamma ,$ H : A $\wedge$ B , H' : A , H'' : B
$\vdash$ p : C}
\RightLabel{\quad ($\wedge$L)}
\UnaryInfC{$\psi ; \Gamma ,$ H : A $\wedge$ B $\vdash$
let ([H'],[H'']) = [H] in p : C}
\DisplayProof
\]

\[
\AxiomC{$\psi ; \Gamma \vdash$ p : A}
\AxiomC{$\psi ; \Gamma \vdash$ q : B}
\RightLabel{\quad ($\wedge$R)}
\BinaryInfC{$\psi ; \Gamma \vdash$ (p , q) : A $\wedge$ B}
\DisplayProof
\]

Disjunction:
\[
\AxiomC{$\psi ; \Gamma$ , H : A $ \vee$ B , H' : A $\vdash$ p : C}
\AxiomC{$\psi ; \Gamma$ , H : A $ \vee$ B , H'' : B $\vdash$ q : C}
\RightLabel{\quad ($\vee$L)}
\BinaryInfC{$\psi ; \Gamma ,$  H : A
$ \vee$ B $\vdash $
 match [H] with(
 A [H']: p
 | B [H'']: q ) : C
}
\DisplayProof
\]

\[
\AxiomC{$\psi ; \Gamma \vdash$ p : A}
\RightLabel{\quad ($\vee R_1$)}
\UnaryInfC{$\psi ; \Gamma \vdash$ Left p : A $\vee$ B}
\DisplayProof
\]

\[
\AxiomC{$\psi ; \Gamma \vdash$ q : B}
\RightLabel{\quad ($\vee R_2$)}
\UnaryInfC{$\psi ; \Gamma \vdash$ Right q :  A $\vee$ B}
\DisplayProof
\]

Implication:
\[
\AxiomC{$\psi ; \Gamma ,$ H : A $\supset$ B $\vdash$ p : A}
\AxiomC{$\psi ; \Gamma ,$ H : A $\supset$ B , H' : B $\vdash$ q : C}
\RightLabel{\quad ($\supset$L)}
\BinaryInfC{$\psi ; \Gamma ,$ H : A $\supset$ B $\vdash$
(p, B [ H' ] via [H], q) : C}
\DisplayProof
\]

\[
\AxiomC{$\psi ; \Gamma$ , H : A $\vdash$ p : B}
\RightLabel{\quad ($\supset$R)}
\UnaryInfC{$\psi ; \Gamma \vdash$ ( Assume A [H] , p ) : A
$\supset$ B}
\DisplayProof
\]

Using hypotheses:

\[
\AxiomC{}
\RightLabel{\quad (by)}
\UnaryInfC{$\psi ; \Gamma , $ H : A $\vdash$ by [H] : A}
\DisplayProof
\]

\[
\AxiomC{$\psi ; \Gamma \vdash$ p : A}
\RightLabel{\quad (therefore)}
\UnaryInfC{$\psi ; \Gamma \vdash$ p Therefore A : A}
\DisplayProof
\]

\subsection{Function signature}
\begin{center}
{\tt
check_proof : $\psi \rightarrow \Gamma \rightarrow $ P
$\rightarrow$ A $\rightarrow$ unit option
}
\end{center}

\section{Quantifiers in proofs}

\subsection{Rules}
Existentials:

\[
\AxiomC{$\psi ; \Gamma \vdash$ t : $\tau$}
\AxiomC{$\psi ; \Gamma \vdash$ p : [x $\mapsto$ t] A }
\RightLabel{\quad ($\exists$ R)}
\BinaryInfC{$\psi ; \Gamma \vdash$ Choose t ; p : $\exists x : \tau . $A}
\DisplayProof
\]

\[
\AxiomC{$\psi, y:\tau ; \Gamma, $ H $:\exists x : \tau . A, $ H': $[x \mapsto y] A \vdash$ p : C}
\RightLabel{\quad ($\exists$ L)}
\UnaryInfC{$\psi ; \Gamma , $ H $:\exists x:\tau. $ A $ \vdash$
let ($y$,H') = H in p : C}
\DisplayProof
\]

Universals:
\[
\AxiomC{$\psi , y : \tau  ; \Gamma , $ $\vdash$ p : [$x \mapsto y$] A}
\RightLabel{\quad ($\forall$ R)}
\UnaryInfC{$\psi ; \Gamma \vdash$ Assume $y:\tau$ . p : $\forall x : \tau . A $}
\DisplayProof
\]

\[
\AxiomC{$\psi ; \Gamma \vdash$ t : $\tau$}
\AxiomC{$\psi ; \Gamma$ ,
H : $\forall x : \tau $ . A ,
H' : [x $\mapsto$ t] A  $\vdash$ p : C}
\RightLabel{\quad ($\forall$ L)}
\BinaryInfC{$\psi ; \Gamma , $ H $:\forall x:\tau. $ A $ \vdash$
let H' = H with t in p : C}
\DisplayProof
\]

\subsection{Substituting terms into variables}

\begin{center}
{\tt
subs = $[x \mapsto z]$
}
\end{center}

\begin{center}
{\tt
\begin{tabular}{rl}
subs_term &: $x \rightarrow $ t $ \rightarrow $ t $\rightarrow$ t
\\
subs_prop &: $x\rightarrow$ t $\rightarrow$ A $\rightarrow[x]\rightarrow$ A
\end{tabular}
}
\end{center}

\begin{center}
{\tt
\begin{tabular}{rl}
val subs_term &: var -> term -> term -> term
\\
val subs_prop &: var -> term -> prop -> var list -> prop
\end{tabular}
}
\end{center}

\section{$\boldsymbol \alpha$-equivalence}
\subsection{Terms}

Variables:
\[
\AxiomC{}
\RightLabel{\quad (var$\overset{\alpha}=$)}
\UnaryInfC{$x$ $\overset{\alpha}=$ $x$}
\DisplayProof
\]

Booleans:
\[
\AxiomC{}
\RightLabel{\quad (bool-true$\overset{\alpha}=$)}
\UnaryInfC{true $\overset{\alpha}=$ true}
\DisplayProof
\quad
\quad
\AxiomC{}
\RightLabel{\quad (bool-false$\overset{\alpha}=$)}
\UnaryInfC{false $\overset{\alpha}=$ false}
\DisplayProof
\]

Natural Numbers:
\[
\AxiomC{}
\RightLabel{\quad (nat-zero$\overset{\alpha}=$)}
\UnaryInfC{zero $\overset{\alpha}=$ zero}
\DisplayProof
\quad
\quad
\AxiomC{t  $\overset{\alpha}=$  t'}
\RightLabel{\quad (nat-suc-n$\overset{\alpha}=$)}
\UnaryInfC{suc( t ) $\overset{\alpha}=$ suc( t' )}
\DisplayProof
\]

Lists:
\[
\AxiomC{}
\RightLabel{\quad (list-nil$\overset{\alpha}=$)}
\UnaryInfC{[] $\overset{\alpha}=$ []}
\DisplayProof
\quad
\quad
\AxiomC{e  $\overset{\alpha}=$  e'}
\AxiomC{v  $\overset{\alpha}=$  v'}
\RightLabel{\quad (list-cons$\overset{\alpha}=$)}
\BinaryInfC{e::v $\overset{\alpha}=$ e'::v'}
\DisplayProof
\]

Application:
\[
\AxiomC{e $\overset{\alpha}=$ e'}
\AxiomC{v $\overset{\alpha}=$ v'}
\RightLabel{\quad (var$\overset{\alpha}=$)}
\BinaryInfC{e v $\overset{\alpha}=$ e' v'}
\DisplayProof
\]

\subsection{Propositions}
Truth and Falsity:
\[
\AxiomC{}
\RightLabel{\quad ($\top\overset{\alpha}=$)}
\UnaryInfC{$\top \overset{\alpha}= \top$}
\DisplayProof
\quad
\quad
\AxiomC{}
\RightLabel{\quad ($\bot\overset{\alpha}=$)}
\UnaryInfC{$\bot \overset{\alpha}= \bot$}
\DisplayProof
\]

Binary Relations:
\[
\AxiomC{A $\overset{\alpha}=$ A'}
\AxiomC{B $\overset{\alpha}=$ B'}
\RightLabel{\quad ($\wedge\overset{\alpha}=$)}
\BinaryInfC{ A $\wedge$ B $\overset{\alpha}=$ A' $\wedge$ B'}
\DisplayProof
\]

\[
\AxiomC{A $\overset{\alpha}=$ A'}
\AxiomC{B $\overset{\alpha}=$ B'}
\RightLabel{\quad ($\vee\overset{\alpha}=$)}
\BinaryInfC{ A $\vee$ B $\overset{\alpha}=$ A' $\vee$ B'}
\DisplayProof
\]

\[
\AxiomC{A $\overset{\alpha}=$ A'}
\AxiomC{B $\overset{\alpha}=$ B'}
\RightLabel{\quad ($\supset\overset{\alpha}=$)}
\BinaryInfC{ A $\supset$ B $\overset{\alpha}=$ A' $\supset$ B'}
\DisplayProof
\]

Equality:
\[
\AxiomC{t$_1$ $\overset{\alpha}=$ t$_1'$}
\AxiomC{t$_2$ $\overset{\alpha}=$ t$_2'$}
\AxiomC{$\tau$ $\overset{\alpha}=$ $\tau$'}
\RightLabel{\quad ($=\overset{\alpha}=$)}
\TrinaryInfC{ (t$_1$ = t$_2$ : $\tau$) $\overset{\alpha}=$ (t$_1$' = t$_2$' : $\tau$')}
\DisplayProof
\]

Quantifiers:
\[
\AxiomC{$\new$ $z$ . $(x$ $z)$ B $\overset{\alpha}=$ $(x$ $z)$ B'}
\AxiomC{$\tau \overset{\alpha}= \tau'$}
\RightLabel{\quad ($\exists\overset{\alpha}=$)}
\BinaryInfC{$\exists x : \tau$. B $\overset{\alpha}=$ $\exists y : \tau' $. B' }
\DisplayProof
\]

\[
\AxiomC{$\new$ $z$ . $(x$ $z)$ B $\overset{\alpha}=$ $(x$ $z)$ B'}
\AxiomC{$\tau \overset{\alpha}= \tau'$}
\RightLabel{\quad ($\forall\overset{\alpha}=$)}
\BinaryInfC{$\forall x : \tau$. B $\overset{\alpha}=$ $\forall y : \tau' $. B' }
\DisplayProof
\]

\subsection{Swapping variable names}

\begin{center}
{\tt
swap = $(x$ $z)$
}
\end{center}

\begin{center}
{\tt
\begin{tabular}{rl}
swap_term &: $x \rightarrow z \rightarrow $ t $\rightarrow$ t
\\
swap_prop &: $x \rightarrow z \rightarrow $ A $\rightarrow$ A
\end{tabular}
}
\end{center}

\begin{center}
{\tt
\begin{tabular}{rl}
val swap_term &: var -> var -> term -> term
\\
val swap_prop &: var -> var -> prop -> prop
\end{tabular}
}
\end{center}

\section{Induction in proofs}

\subsection{Rules through predicates}

Natural Numbers:
\[
\AxiomC{
$\psi ; \Gamma \vdash$ p : P(zero)
}
\AxiomC{
$\psi$ , $n$ : nat ; $\Gamma$ , H : P($n$) $\vdash$ q : P(suc($n$))
}
\RightLabel{\quad (induction-nat)}
\BinaryInfC{
$\psi ; \Gamma$ $\vdash$
(Induction on nat: case zero : p ; case suc($n$) : [H] , q)
: ($\forall$ $m$ : nat . P($m$))
}
\DisplayProof
\]

Lists:
\[
\AxiomC{
$\psi ; \Gamma \vdash$ p : P( [] )
}
\AxiomC{
$\psi$ , $x$ : $\tau$ , $xs$ : list $\tau$ ;
$\Gamma$ , H : P($xs$) $\vdash$ q : P($x$ :: $xs$)
}
\RightLabel{\quad (induction-list)}
\BinaryInfC{
$\psi ; \Gamma$ $\vdash$
(Induction on list: case [] : p ; case ($x$ :: $xs$) : [H] , q)
: ($\forall$ $ys$ : list $\tau$ . P($ys$))
}
\DisplayProof
\]

Booleans:
\[
\AxiomC{
$\psi ; \Gamma \vdash$ p : P( true )
}
\AxiomC{
$\psi ; \Gamma \vdash$ q : P( false )
}
\RightLabel{\quad (induction-bool)}
\BinaryInfC{
$\psi ; \Gamma \vdash$
(Induction on bool: case true : p ; case false : q )
: ($\forall$ $b$ : bool . P( $b$ ))
}
\DisplayProof
\]

\subsection{Rules through substitution}

Natural Numbers:
\[
\AxiomC{
$\psi ; \Gamma \vdash$ p : [$m$ $\mapsto$ zero] C
}
\AxiomC{
$\psi$ , $n$ : nat ; $\Gamma$ , H : [$m$ $\mapsto$ zero] C $\vdash$ q : [m $\mapsto$ suc($n$)] C
}
\RightLabel{\quad (induction-nat)}
\BinaryInfC{
$\psi ; \Gamma$ $\vdash$
(Ind-Nat: zero : p ; suc($n$) : [H] , q)
: ($\forall$ $m$ : nat . C)
}
\DisplayProof
\]

Lists:
\[
\AxiomC{
$\psi ; \Gamma \vdash$ p : [$ys$ $\mapsto$ [] ] C
}
\AxiomC{
$\psi$ , $x$ : $\tau$ , $xs$ : list $\tau$ ;
$\Gamma$ , H : [$ys$ $\mapsto$ $xs$ ] C $\vdash$ q : [$ys$ $\mapsto$ $x$ :: $xs$ ] C
}
\RightLabel{\quad (induction-list)}
\BinaryInfC{
$\psi ; \Gamma$ $\vdash$
(Ind-List: [] : p ; ($x$ :: $xs$) : [H] , q)
: ($\forall$ $ys$ : list $\tau$ . C)
}
\DisplayProof
\]

Booleans:
\[
\AxiomC{
$\psi ; \Gamma \vdash$ p : [$b$ $\mapsto$ true ] C
}
\AxiomC{
$\psi ; \Gamma \vdash$ q : [$b$ $\mapsto$ false ] C
}
\RightLabel{\quad (induction-bool)}
\BinaryInfC{
$\psi ; \Gamma \vdash$
(Ind-Bool: true : p ; false : q )
: ($\forall$ $b$ : bool . C)
}
\DisplayProof
\]

\section{Equality in proofs}

\subsection{Abstract congruence closure \cite[p.~4--7]{BachmairTV03}}

\subsubsection{Definition}


Rewrite-Rules:
\begin{align*}
D\text{-}rule : &&f(c_0, ... c_k) \rightarrow c &&&\textit{where $f$ is a term constructor and $c_i$ are constants in $K$}
\\
C\text{-}rule : &&c \rightarrow d &&&\textit{where $c$ and $d$ are constants in $K$}
\end{align*}
Sets:
\begin{align*}
D &: \{D\text{-}rule\}\\
C &: \{C\text{-}rule\}
\end{align*}
\begin{align*}
E &: \{(t = t) : \tau\}\\
K &: \{ x \mid x \notin E\}\\
R &: D \cup C\\
\end{align*}
Closure Construction:
\[state : (K,E,R)\]
\[
\AxiomC{$(\emptyset , E , \emptyset)$}
\LeftLabel{{\tt build\_acc}: \quad}
\RightLabel{\quad \it where $R$ is the abstract congruence closure (ACC) of $E$}
\UnaryInfC{$(K , \emptyset , R)$}
\DisplayProof
\]

\subsubsection{Sate transition rules}

\[
\AxiomC{$(K,E[t],R)$}
\AxiomC{$t = f(c_0 , ... , c_k)$}
\AxiomC{$c_i \in K$ $\wedge$ $c \notin K$}
\LeftLabel{Extension: \quad}
\RightLabel{\quad (Ext)}
\TrinaryInfC{$(K \cup \{c\},E[c],R \cup \{t \rightarrow c\ : D\})$}
\DisplayProof
\]

\[
\AxiomC{$(K,E[t],R \cup \{t \rightarrow c : D\})$}
\LeftLabel{Simplification: \quad}
\RightLabel{\quad (Sim)}
\UnaryInfC{$(K,E[c],R \cup \{t \rightarrow c : D\})$}
\DisplayProof
\]

\[
\AxiomC{$(K \cup \{c\},E \cup \{t = c \},R\})$}
\LeftLabel{Orientation1: \quad}
\RightLabel{\quad (Ori1)}
\UnaryInfC{$(K \cup \{c\},E,R \cup \{t \rightarrow c : D\})$}
\DisplayProof
\]

\[
\AxiomC{$(K \cup \{c,d\},E \cup \{c = d \},R\})$}
\AxiomC{$c < d$}
\LeftLabel{Orientation2: \quad}
\RightLabel{\quad (Ori2)}
\BinaryInfC{$(K \cup \{c,d\},E,R \cup \{c \rightarrow d : C\})$}
\DisplayProof
\]

\[
\AxiomC{$(K \cup \{c,d\},E \cup \{c = d \},R\})$}
\AxiomC{$d < c$}
\LeftLabel{Orientation3: \quad}
\RightLabel{\quad (Ori2)}
\BinaryInfC{$(K \cup \{c,d\},E,R \cup \{d \rightarrow c : C\})$}
\DisplayProof
\]

\[
\AxiomC{$(K,E \cup \{t = t \},R\})$}
\LeftLabel{Deletion: \quad}
\RightLabel{\quad (Del)}
\UnaryInfC{$(K,E,R\})$}
\DisplayProof
\]

\[
\AxiomC{$(K,E,R \cup \{t \rightarrow c : D , t \rightarrow d : D \})$}
\LeftLabel{Deduction1: \quad}
\RightLabel{\quad (Ded1)}
\UnaryInfC{$(K,E \cup \{c = d \},R \cup \{t \rightarrow d : D\})$}
\DisplayProof
\]

\[
\AxiomC{$(K,E,R \cup \{c \rightarrow c' : C , c \rightarrow d : C \})$}
\LeftLabel{Deduction2: \quad}
\RightLabel{\quad (Ded2)}
\UnaryInfC{$(K,E \cup \{c' = d \},R \cup \{c \rightarrow d : C\})$}
\DisplayProof
\]

\[
\AxiomC{$(K,E,R \cup \{s[c] \rightarrow c' : D , c \rightarrow d : C \})$}
\LeftLabel{Collapse: \quad}
\RightLabel{\quad (Col)}
\UnaryInfC{$(K,E,R \cup \{s[d] \rightarrow c' : D , c \rightarrow d : C \})$}
\DisplayProof
\]

\[
\AxiomC{$(K,E,R \cup \{t \rightarrow c : D , c \rightarrow d : C \})$}
\LeftLabel{Composition: \quad}
\RightLabel{\quad (Com)}
\UnaryInfC{$(K,E,R \cup \{t \rightarrow d : D , c \rightarrow d : C \})$}
\DisplayProof
\]

\subsection{Equality through congruence}

\[
\AxiomC{$\psi~ ;~ \Gamma ~\vdash~$ H$_i$ : $(t_i = t_i ') : \tau_i$}
\AxiomC{$\forall i \in \{1 ... n\}~ . ~ \overset{\xrightharpoonup{~~~~~~~~}}{t_i = t_i '} ~\vDash~ t = t'$}
\RightLabel{\quad (eq)}
\BinaryInfC{$\psi~ ;~ \Gamma ~\vdash~$ By Equality ( H$_0$ , ... , H$_n$ ) : ($t = t' : \tau$)}
\DisplayProof
\]

\section{Spine application and hypotheses labelling}

\subsection{Rules for proofs}

\begin{center}
\begin{tabular}{rrl}

(simple-proofs) & \quad spf ::=& [H] with s $\mid$ By [H] $\mid$ Left spf $\mid$  Right spf $\mid$ (spf , spf) $\mid$ tt
\\
(proofs) & \quad p ::=& ... $\mid$ [H] with s $\mid$ We know [H] : A because spf , p
\\
(spines) & \quad s ::=& . $\mid$ [H] , s $\mid$ t , s

\end{tabular}
\end{center}

\begin{center}
\begin{tabular}{rll}

{\tt check_simple_pf} &::& {\tt spf} $\rightarrow$ {\tt unit option}

\end{tabular}
\end{center}

\[
\AxiomC{$\psi ; \Gamma $ $\vdash$ spf : A}
\AxiomC{$\psi ; \Gamma ,$ H : A $\vdash$ p : C}
\LeftLabel{Labelling: \quad}
\RightLabel{\quad (hyp-label)}
\BinaryInfC{$\psi ; \Gamma $ $\vdash$ We know [H] : A because spf , p : C}
\DisplayProof
\]

\[
\AxiomC{$\overset{-}\psi ; \overset{-}\Gamma ,$ H : A $\vdash$ $\overset{-}{\text s}$ : $\overset{-}{\text A}$ $\gg$ $\overset{+}{\text B}$}
\AxiomC{B $\overset{\alpha}=$ C}
\LeftLabel{Spine application: \quad}
\RightLabel{\quad (spine-app)}
\BinaryInfC{$\psi ; \Gamma $, H : A $\vdash$ [H] with s : C}
\DisplayProof
\]

\subsection{Rules for spline application}

Rules:
\[
\AxiomC{}
\AxiomC{}
\RightLabel{\quad (id-spine-app)}
\BinaryInfC{$\psi ; \Gamma $ $\vdash$ . : A $\gg$ A}
\DisplayProof
\]

\[
\AxiomC{[H] : A' $\in$ $\Gamma$}
\AxiomC{$\psi ; \Gamma $ $\vdash$ s : B $\gg$ C}
\AxiomC{A $\overset{\alpha}=$ A'}
\RightLabel{\quad ($\supset$-spine-app)}
\TrinaryInfC{$\psi ; \Gamma $ $\vdash$ [H] , s : A $\supset$ B $\gg$ C}
\DisplayProof
\]

\[
\AxiomC{$\psi \vdash$ t : $\tau$}
\AxiomC{$\psi ; \Gamma $ $\vdash$ s : [t $\mapsto$ x] A $\gg$ C}
\RightLabel{\quad ($\forall$-spine-app)}
\BinaryInfC{$\psi ; \Gamma $ $\vdash$ t , s : $\forall x :\tau$ . A $\gg$ C}
\DisplayProof
\]

Function signatures:

\begin{center}
\begin{tabular}{rll}

{\tt apply_spine} &::& $\psi$ $\rightarrow$ $\Gamma$ $\rightarrow$ s $\rightarrow$ A $\rightarrow$ B {\tt option}
\\
{\tt apply_spine} &::& {\tt ctx} $\rightarrow$ {\tt hyps} $\rightarrow$ {\tt spine} $\rightarrow$ {\tt prop} $\rightarrow$ {\tt prop option}

\end{tabular}
\end{center}

\section{Error handling}

\subsection{Adding lexical position data}

\begin{center}
\begin{tabular}{llrl}
(term') &t' &:=& $x$ $\mid$ t t $\mid$ true $\mid$ false $\mid$ Zero $\mid$ Suc t $\mid$ Cons (t,t)\\
(term) &t &:=& (pos, pos) , t'\\
\\
(prop') &A' &:=& $\top$ $\mid$ $\bot$ $\mid$ A $\wedge$ A $\mid$ A $\vee$ A $\mid$ A $\supset$ A $\mid$ t $=$ t : $\tau$ $\mid$ $\forall x$ . p $\mid$ $\exists x$ . p\\
(prop) &A &:=& (pos, pos) , A'\\
\\
(proof') &p' &:=& tt $\mid$ Absurd $\mid$ ... \\
(proof) &p &:=& (pos, pos) , p'\\
\end{tabular}
\end{center}

\subsection{Monadic return type}

\subsubsection{Return type}

\subsubsection{Monadic operations}

\subsection{Optional hypotheses label annotations}



\bibliography{notes}
\bibliographystyle{plain}

\end{document}